theories/GuardError.v
@@ -1,0 +1,47 @@
+From MetaCoq.Utils Require Import utils.
+From MetaCoq.Template Require Import Ast.
+From MetaCoq.Guarded Require Export Trace.
+
+(** Exceptions *)
+(** most of the code runs in a monad for handling errors/exceptions *)
+Declare Scope exc_scope.
+Open Scope exc_scope.
+
+Notation loc := string (only parsing).
+
+(** TODO YJ: what do the parameters mean? *)
+Inductive fix_guard_error :=
+  | NotEnoughAbstractionInFixBody
+  | RecursionNotOnInductiveType : term -> fix_guard_error
+  | RecursionOnIllegalTerm : nat -> (context * term) -> (list nat * list nat) -> fix_guard_error
+  | NotEnoughArgumentsForFixCall : nat -> fix_guard_error
+  | FixpointOnIrrelevantInductive.
+
+Inductive guard_exc := 
+  | ProgrammingErr (w : loc) (s : string)
+  | OtherErr (w : loc) (s : string)
+  | EnvErr (w: loc) (kn : kername) (s : string)
+  | IndexErr (w : loc) (s : string) (i : nat)
+  | GuardErr (w : loc) (s : string) (e : fix_guard_error)
+  | PositivityError (w : loc) (s : string)
+  | TimeoutErr
+  | NoReductionPossible. 
+
+(*max bind steps *)
+Definition max_steps := 1000. 
+Definition catchE := @catchE max_steps. 
+Arguments catchE {_ _}. 
+Definition catchMap := @catchMap max_steps _ TimeoutErr. 
+Arguments catchMap {_ _}. 
+  
+Instance trace_monad : Monad (@TraceM guard_exc).
+apply trace_monad. exact max_steps. exact TimeoutErr.
+Defined.
+
+(* Notation "'exc' A" := (excOn guard_exc A) (at level 100) : exc_scope.  *)
+Notation "'exc' A" := (@TraceM guard_exc A) (at level 100) : exc_scope. 
+(* Definition unwrap := @exc_unwrap. *)
+Definition unwrap := @trc_unwrap.
+Arguments unwrap { _ _ _ _}. 
+
+Instance: TrcUnwrap list := list_trc_unwrap max_steps TimeoutErr.
