theories/MCRTree.v
@@ -1,11 +1,11 @@
 (* Type of regular trees:
-   - Param denotes tree variables (like de Bruijn indices) ()
+   - Var denotes tree variables (like de Bruijn indices) ()
      the first int is the depth of the occurrence (YJ: in nested inductive types),
      and the second int is the index in the array of trees introduced at that depth
      (YJ: index in mutual inductive types).
-     ==============================================================================    Warning: Param's indices both start at 0!!!
+     ==============================================================================    Warning: Var's indices both start at 0!!!
    - Node denotes the usual tree node, labelled with X (YJ: exclusively recargs
-      in the current implementation. [children] contains [Param]s, one for each
+      in the current implementation. [children] contains [Var]s, one for each
       constructor.)
 
    - Rec(j,v1..vn) introduces an infinite tree. It denotes v(j+1) with
@@ -21,35 +21,34 @@
     a singleton [Node].)
  *)
 Inductive rtree (X : Type) :=
-  | Param (tree_index : nat) (ind_index : nat)
-  | Node (l : X) (children : list (rtree X))
+  | Var (tree_index : nat) (ind_index : nat)
+  | Node (l : X) (children : list (list (rtree X)))
   | Rec (index : nat) (children : list (rtree X)).
 
-Arguments Param {_}.
+Arguments Var {_}.
 Arguments Node {_}.
 Arguments Rec {_}.
 
-Require Import List.
+Require Import List Nat.
 Import ListNotations.
-Require Import Coq.Lists.ListSet.
-Require Import Coq.Arith.PeanoNat.
-From MetaCoq.Utils Require Import MCUtils.
-From MetaCoq.Guarded Require Import util.
+From MetaCoq.Utils Require Import MCUtils monad_utils.
+From MetaCoq.Guarded Require Import util GuardError.
 
 (* TODO: proper exception handling with the except monad *)
 
 Open Scope bool_scope.
+Open Scope nat_scope.
 
 Unset Guard Checking.
 Section trees.
 Context {X : Type}.
 Implicit Types (t : rtree X).
 
-Definition default_tree := Param (X:=X) 0 0. (* bogus tree used as default value*)
+Definition default_tree := Var (X:=X) 0 0. (* bogus tree used as default value*)
 
 (* Building trees *)
 (* array of "references" to mutual inductives of innermostly introduced (by Rec) inductive *)
-Definition mk_rec_calls i := tabulate (fun j => Param (X := X) 0 j) i.
+Definition mk_rec_calls i := tabulate (fun j => Var (X := X) 0 j) i.
 
 Definition mk_node label children := Node (X := X) label children.
 
@@ -57,10 +56,10 @@ Definition mk_node label children := Node (X := X) label children.
 (* lift unbound references >= depth to inductive types by n *)
 Fixpoint lift_rtree_rec depth n (t : rtree X) :=
   match t with
-  | Param i j =>
+  | Var i j =>
       (* lift all but the innermost depth types by n *)
-      if i <? depth then t else Param (i+n) j
-  | Node l children => Node l (map (lift_rtree_rec depth n) children)
+      if i <? depth then t else Var (i+n) j
+  | Node l children => Node l (map (map (lift_rtree_rec depth n)) children)
   | Rec j defs => Rec j (map (lift_rtree_rec (S depth) n) defs)
   end.
 
@@ -72,27 +71,30 @@ Definition rtree_lift n t := if n =? 0 then t else lift_rtree_rec 0 n t.
 (* substitute the depth -th unbound type by sub *)
 Fixpoint subst_rtree_rec depth sub t :=
   match t with
-  | Param i j as t =>
+  | Var i j as t =>
       if i <? depth then t
       else if i =? depth then  (* we refer to the inductive, depth, we want to substitute *)
         rtree_lift depth (Rec j sub) (* substitute in and lift references in sub by depth in order to avoid capture *)
-      else Param (i-1) j
-  | Node l children => Node l (map (subst_rtree_rec depth sub) children)
+      else Var (i-1) j
+  | Node l children => Node l (map (map (subst_rtree_rec depth sub)) children)
   | Rec j defs => Rec j (map (subst_rtree_rec (S depth) sub) defs)
   end.
 
 (* substitute the innermost unbound by sub *)
 Definition subst_rtree sub t := subst_rtree_rec 0 sub t.
 
-(* To avoid looping, we must check that every body introduces a node
-   or a parameter *)
-Fixpoint expand t :=
+Import MCMonadNotation.
+Open Scope bs.
+(* To avoid looping, we must check that every body introduces a node or a var *)
+Fixpoint expand t : exc (rtree X) :=
   match t with
-  | Rec j defs => expand (subst_rtree defs (nth j defs default_tree)) (* substitute by the j-th inductive type declared here *)
-  | t => t
+  | Rec j defs =>
+      def <- except (IndexErr "MCRTree::expand" "" j) (nth_error defs j) ;;
+      expand (subst_rtree defs def) (* substitute by the j-th inductive type declared here *)
+  | t => ret t
   end.
 (* loops on some inputs:*)
-(*Fail Timeout 1 Compute(expand (Rec 0 [(Param 0 0)])). *)
+(*Fail Timeout 1 Compute(expand (Rec 0 [(Var 0 0)])). *)
 
 
 (* Given a vector of n bodies, builds the n mutual recursive trees.
@@ -104,7 +106,7 @@ Fixpoint expand t :=
 Definition mk_rec defs :=
   let check := fix rec (histo : set nat) d {struct d} :=
     match expand d with
-    | Param 0 j =>
+    | Var 0 j =>
         if set_mem (Nat.eq_dec) j histo
         then None (* invalid recursive call *)
         else
@@ -122,7 +124,7 @@ Definition mk_rec defs :=
 (* Tree destructors, expanding loops when necessary *)
 Definition destruct_param {Y} t (f : nat -> nat -> Y) y :=
   match expand t with
-  | Param i j => f i j
+  | Var i j => f i j
   | _ => y
   end.
 Definition destruct_node {Y} t (f : X -> list (rtree X) -> Y) y :=
@@ -142,7 +144,7 @@ Definition is_node t :=
 
 Fixpoint map_rtree {Y} (f : X -> Y) t :=
   match t with
-  | Param i j => Param i j
+  | Var i j => Var i j
   | Node a children => Node (f a) (map (map_rtree f) children)
   | Rec j defs => Rec j (map (map_rtree f) defs)
   end.
@@ -150,7 +152,7 @@ Fixpoint map_rtree {Y} (f : X -> Y) t :=
 (** Structural equality test, parametrized by an equality on elements *)
 Definition rtree_eqb (eqbX : X -> X -> bool) := fix rec t t' :=
   match t, t' with
-  | Param i j, Param i' j' => Nat.eqb i i' && Nat.eqb j j'
+  | Var i j, Var i' j' => Nat.eqb i i' && Nat.eqb j j'
   | Node x c, Node x' c' => eqbX x x' && list_eqb rec c c'
   | Rec i a, Rec i' a' => Nat.eqb i i' && list_eqb rec a a'
   | _, _ => false
@@ -180,10 +182,10 @@ Definition rtree_equal eqb t t' := rtree_eqb eqb t t' || rtree_equiv eqb eqb t t
 (* n is the Rec nesting level *)
 Definition rtree_inter' (eqb : X -> X -> bool) (interlbl : X -> X -> option X) def := fix rec n (histo : list ((rtree X * rtree X) * (nat * nat))) t t' {struct t} : option (rtree X):=
   match lookup (pair_eqb (rtree_eqb eqb)) (t, t') histo with
-  | Some (i, j) => Some (Param (n - i - 1) j)
+  | Some (i, j) => Some (Var (n - i - 1) j)
   | None =>
       match t, t' with
-      | Param i j, Param i' j' =>
+      | Var i j, Var i' j' =>
           if Nat.eqb i i' && Nat.eqb j j' then Some t else None
       | Node x a, Node x' a' =>
           match interlbl x x' with
